Reorganize theories

HoTT_Base.thy
@@ -1,8 +1,8 @@
 (*  Title:  HoTT/HoTT_Base.thy
     Author: Josh Chen
-    Date:   Jun 2018
+    Date:   Aug 2018
 
-Basic setup and definitions of a homotopy type theory object logic.
+Basic setup and definitions of a homotopy type theory object logic with a cumulative universe hierarchy à la Russell.
 *)
 
 theory HoTT_Base
@@ -12,71 +12,77 @@ begin
 
 section \<open>Foundational definitions\<close>
 
-text "A single meta-type \<open>Term\<close> suffices to implement the object-logic types and terms."
+text "Meta syntactic type for object-logic types and terms."
 
 typedecl Term
 
 
-section \<open>Named theorems\<close>
-
-text "Named theorems to be used by proof methods later (see HoTT_Methods.thy).
-
-\<open>wellform\<close> declares necessary wellformedness conditions for type and inhabitation judgments, while
-\<open>comp\<close> declares computation rules, which are used by the simplification method as equational rewrite rules."
-
-named_theorems wellform
-named_theorems comp
-
-
 section \<open>Judgments\<close>
 
-text "Formalize the context and typing judgments  \<open>a : A\<close>.
-
-For judgmental equality we use the existing Pure equality \<open>\<equiv>\<close> and hence do not need to define a separate judgment for it."
+text "
+  Formalize the typing judgment \<open>a : A\<close>.
+  For judgmental/definitional equality we use the existing Pure equality \<open>\<equiv>\<close> and hence do not need to define a separate judgment for it.
+"
 
 consts
-  is_of_type :: "[Term, Term] \<Rightarrow> prop"  ("(1_ : _)" [0, 0] 1000)
+  has_type :: "[Term, Term] \<Rightarrow> prop"  ("(1_ : _)" [0, 0] 1000)
 
 
-section \<open>Universes\<close>
+section \<open>Universe hierarchy\<close>
 
-text "Strictly-ordered meta-level natural numbers to index the universes."
+text "Finite meta-ordinals to index the universes."
 
-typedecl Numeral
+typedecl Ord
 
 axiomatization
-  O :: Numeral ("0") and
-  S :: "Numeral \<Rightarrow> Numeral" ("S_") and
-  lt :: "[Numeral, Numeral] \<Rightarrow> prop"  (infix "<-" 999)
+  O :: Ord and
+  S :: "Ord \<Rightarrow> Ord"  ("S_" [0] 1000) and
+  lt :: "[Ord, Ord] \<Rightarrow> prop"  (infix "<-" 999)
 where
-  Numeral_lt_min: "\<And>n. 0 <- S n"
+  Ord_lt_min: "\<And>n. O <- S n"
 and
-  Numeral_lt_trans: "\<And>m n. m <- n \<Longrightarrow> S m <- S n"
+  Ord_lt_trans: "\<And>m n. m <- n \<Longrightarrow> S m <- S n"
 
-lemmas Numeral_rules [intro] = Numeral_lt_min Numeral_lt_trans
+lemmas Ord_rules [intro] = Ord_lt_min Ord_lt_trans
   \<comment> \<open>Enables \<open>standard\<close> to automatically solve inequalities.\<close>
 
-text "Universe types:"
+text "Define the universe types."
 
 axiomatization
-  U :: "Numeral \<Rightarrow> Term"  ("U _")
+  U :: "Ord \<Rightarrow> Term"
 where
-  Universe_hierarchy: "\<And>i j. i <- j \<Longrightarrow> U(i) : U(j)"
+  U_hierarchy: "\<And>i j. i <- j \<Longrightarrow> U(i) : U(j)"
 and
-  Universe_cumulative: "\<And>A i j. \<lbrakk>A : U(i); i <- j\<rbrakk> \<Longrightarrow> A : U(j)"
-  \<comment> \<open>WARNING: \<open>rule Universe_cumulative\<close> can result in an infinite rewrite loop!\<close>
+  U_cumulative: "\<And>A i j. \<lbrakk>A : U(i); i <- j\<rbrakk> \<Longrightarrow> A : U(j)"
+    \<comment> \<open>WARNING: \<open>rule Universe_cumulative\<close> can result in an infinite rewrite loop!\<close>
 
 
 section \<open>Type families\<close>
 
-text "We define the following abbreviation constraining the output type of a meta lambda expression when given input of certain type."
+text "
+  The following abbreviation constrains the output type of a meta lambda expression when given input of certain type.
+"
 
-abbreviation (input) constrained :: "[Term \<Rightarrow> Term, Term, Term] \<Rightarrow> prop"  ("_: _ \<longrightarrow> _")
+abbreviation (input) constrained :: "[Term \<Rightarrow> Term, Term, Term] \<Rightarrow> prop"  ("(1_: _ \<longrightarrow> _)")
   where "f: A \<longrightarrow> B \<equiv> (\<And>x. x : A \<Longrightarrow> f x : B)"
 
-text "The above is used to define type families, which are just constrained meta-lambdas \<open>P: A \<longrightarrow> B\<close> where \<open>A\<close> and \<open>B\<close> are elements of some universe type."
+text "
+  The above is used to define type families, which are constrained meta-lambdas \<open>P: A \<longrightarrow> B\<close> where \<open>A\<close> and \<open>B\<close> are small types.
+"
 
 type_synonym Typefam = "Term \<Rightarrow> Term"
+
+
+section \<open>Named theorems\<close>
+
+text "
+  Named theorems to be used by proof methods later (see HoTT_Methods.thy).
+  
+  \<open>wellform\<close> declares necessary wellformedness conditions for type and inhabitation judgments, while \<open>comp\<close> declares computation rules, which are used by the simplification method as equational rewrite rules.
+"
+
+named_theorems wellform
+named_theorems comp
 
 
 end
